# Elementary Number Theory

## The natural numbers

Intuitively, the natural numbers consist of $1, 1 + 1, 1+ 1 + 1, \dots$

How do you know you have captured all natural numbers? How do you know they are all distinct?

We shall assume:

::: {.definition name="Peano Axioms"}

The natural numbers, $\mathbb{N}$, is a set containing a special element '$1$' with an operation '$+1$' satisfying

i. $\forall \; n \in \mathbb{N},\ n + 1 \neq 1$;
ii. $\forall \; m, n \in \mathbb{N},\ \text{ if } m \neq n,\ \text{ then } m + 1 \neq n + 1$
iii. for any property $P(n)$, if $P(1)$ is true and $\forall \; n \in \mathbb{N}, P(n) \implies P(n + 1),$ then $P(n)$ is true for all natural numbers
:::

iii is called the induction axiom.

i and ii capture the idea that any two natural numbers are distinct; iii captures our intuitive notion that the list^[$1, 1 + 1, 1+ 1 + 1, \dots$] is complete (i.e. encompasses all natural numbers).^[to see this rigorously, take $P(n)$ = "$n$ is on this list]

Now we can write 2 for $1 + 1$, 3 for $1 + 1 + 1$, etc, and we can define an operation '$+ k$' for any natural number $k$:
    
$\hspace{1cm}$ for every natural number $n$, we know $n + (k + 1) = (n + k) + 1$;

$\hspace{1cm}$ and so by induction, taking $P(k)$ = "'$+k$' is defined", proved.

Similarly, we can define multiplication, powers, etc. You may check that the "normal" rules of arithmetic apply:

<!--
1. $\forall \; a, b, \in \mathbb{N} \hspace{1cm} a + b = b + a$ [($+$ is commutative);]{style="float:right"}
2. $\forall \; a, b, \in \mathbb{N} \hspace{1.2cm} a b = b a$ ($\times$ is commutative);
3. $\forall \; a, b, c \in \mathbb{N} \hspace{1cm} a + (b + c) = (a + b) + c$ ($+$ is associative);
4. $\forall \; a, b, c \in \mathbb{N} \hspace{1cm} a (b c) = (a b) c$ ($\times$ is associative);
4. $\forall \; a, b, c \in \mathbb{N} \hspace{1cm} a (b + c) = ab + ac$ ($\times$ is distributive over $+$); -->

\begin{align}
    &1.\ \forall \; a, b, \in \mathbb{N}  & &a + b = b + a & &(+ \text{ is commutative}); \\
    &2.\ \forall \; a, b, \in \mathbb{N}  & &ab = ba & &(\times \text{ is commutative}); \\
    &3.\ \forall \; a, b, c \in \mathbb{N} & &a + (b + c) = (a + b) + c & &(+ \text{ is associative}); \\
    &4.\ \forall \; a, b, c \in \mathbb{N} & &a (b c) = (a b) c & &(\times \text{ is associative}); \\
    &5.\ \forall \; a, b, c \in \mathbb{N} & &a (b + c) = ab + ac & &(\times \text{ is distributive over }+);
\end{align} 

We can define $a < b$ if $a + c = b$ for some $c \in \mathbb{N}$. You may want to check

\begin{align}
    &6.\ \forall \; a, b, c & a < b &\implies a + c < b + c \\
    &7.\ \forall \; a, b, c & a < b &\implies a c < b c \\
    &8.\ \forall \; a, b, c & a < b \text{ and } b < c &\implies a < c \\
    &9.\ \forall \; a & &\lnot (a < a).
\end{align} 

Recall the induction axiom: if $P(1)$ holds and $\forall \; n \in \mathbb{N}, P(n) \implies P(n+1)$, then $P(n)$ holds $\forall \; n \in \mathbb{N}$.
This is also known as the *(weak) principle of induction (WPI)*. A more useful form is the *Strong Principle of Induction (SPI)*: if

1. $P(1)$ holds and
2. $\forall \; n \in \mathbb{N}$, we have $P(m) \;\forall \; m \leq n \implies P(n + 1)$, 

then $P(n)$ holds $\forall \; n \in \mathbb{N}$.

In fact, WPI and SPI are equivalent. SPI $\implies$ WPI should be fairly clear. To see WPI $\implies$ SPI, apply the former to $Q(n) = `P(m) \; \forall \; m \leq n'$

*Well-ordering Principle (WOP)*: If $P(n)$ holds for some $n \in \mathbb{N}$, then there is a least $n \in \mathbb{N}$ s.t. $P(n)$ holds.
An alternative phrasing is "every non-empty subset of $\mathbb{N}$ has a minimal element".

::: {.theorem}
SPI is equivalent to the WOP.
:::

::: {.proof}
To show that WOP implies SPI, we assume 1 and 2 from SPI, and show that $P(n)$ holds $\forall \; n \in \mathbb{N}$ using WOP.

Suppose, on the contrary, that $P(n)$ is not true $\forall \; n \in \mathbb{N}$.
Then $C = \{n \in \mathbb{N}: P(n) \text{ is false}\} \neq \emptyset$.
By WOP, $C$ has a minimal element, $m$.
Now $\forall \; k < m$, $k \notin C$ (by minimality of $m$), so $P(k)$ holds $\forall \; k < m$.
But by 2 of SPI, $P(m)$ holds, so contradicting $m \in C$. Hence SPI holds.

To show that SPI implies WOP, suppose there is no least $n \in \mathbb{N}$ s.t. $P(n)$ holds.
We want to show that $P(n)$ does not hold for any $n \in \mathbb{N}$, using SPI.

Consider $Q(n) = `\lnot P(n)'$. 
Certainly $P(1)$ is false (else $1$ would be the minimal element), so $Q(1)$ holds.

Given $n \in \mathbb{N}$, suppose that $Q(k)$ is true $\forall \; k < n$.
Then $P(k)$ is false $\forall \; k < n$.
So $P(n)$ is false as otherwise $n$ would be the minimal element for which $P$ holds.
Hence $Q(n)$ is true, and 2 of SPI holds, so $Q(n)$ is true $\forall \; n \in \mathbb{N}$. 
Thus $P(n)$ is false $\forall \; n \in \mathbb{N}$.
:::

WOP enables us to prove $P(n)$ is true $\forall \; n \in \mathbb{N}$ as follows: If not, then there is a minimal counterexample, and we try and derive a contradiction.

## The integers

The integers, written $\mathbb{Z}$, consist of all symbols $n, -n$, where $n \in \mathbb{N}$, and $0$.

We can define $+$ and $\times$ etc on $\mathbb{Z}$ using $\mathbb{N}$, and check that the usual rules of arithmetic hold.
We also have
\begin{align*}
    &10.\ \forall \; a \in \mathbb{Z} & a + 0 &= a & &(\text{identity for } +) \\
    &11.\ \forall \; a \in \mathbb{Z}, & \exists \; b \in \mathbb{Z} \text{ s.t. } a + b &= 0 & &(\text{inverses for } + ) \\
\end{align*} 

Define '$a < b$' if $a + c = b$ for some $c \in \mathbb{N}$. Rules 6, 8, 9 continue to hold, but 7 must be modified

7'. $\forall \; a, b, c \in \mathbb{Z}, a < b \text{ and } c > 0 \implies ac < bc.$

## The rationals
The rationals, written $\mathbb{Q}$, consist of all expressions $\frac{a}{b}$ (note this is not division as we have not defined division, it just looks the same), where $a, b \in \mathbb{Z}$, $b \neq 0$, and $\frac{a}{b}$ and $\frac{c}{d}$ are regarded as the same if $ad = bc$.

Define $\frac{a}{b} + \frac{c}{d} = \frac{ad + bc}{bd}$, and check it does not matter how we wrote $\frac{a}{b}$ or $\frac{c}{d}$.

We similarly define multiplication, and $`\frac{a}{b} < \frac{c}{d}'$ where $b, d > 0$ if $ad < bc$. 
You can check all preceding rules apply.

In addition
\begin{align*}
    12.\ \forall \; a \in \mathbb{Q},\ a \neq 0,\ \exists \; b \ \text{ s.t. } ab &= 1 & &(\text{inverses for } \times)
\end{align*} 

*Note*. $\mathbb{N} \subset \mathbb{Z} \subset \mathbb{Q}$.

## Primes
Given $a, b \in \mathbb{Z}$ we say "$a$ divides $b$" if $\exists \; c \in \mathbb{Z}$ s.t. $b = ac$. We might also say "$a$ is a divisor/ factor of $b$" or "$b$ is a multiple of $a$". We write $a \mid b$ for $a$ divides $b$.

For any $b \in \mathbb{Z}$, $\pm 1$ and $\pm b$ are always factors; all others are called *proper*.

A natural number $n \geq 2$ is *prime* if its only factors are $\pm 1$ and $\pm n$.^[We don't allow $1$ to be a prime as we want to have unique prime factorisations and it would require every statement to say let $n$ be a prime not equal to $1$.]
If $n \geq 2$ is not prime, then it is *composite*.

::: {.proposition #two}
Every natural number $n \geq 2$ can be written as a product of primes.
:::

::: {.proof}
By induction on $n$. True for $n = 2$.
Let $n > 2$ and suppose that the claim holds up to and including $n - 1$ (SPI). If $n$ is a prime, we are done. If $n$ is composite, then $n = a b$ for some $1 < a, b < n$.
By the induction hypothesis, have $a = p_1 \dots p_k$, $b = q_1 \dots q_l$ for some primes $p_1 \dots p_k, q_1 \dots q_l$.
Hence $n = ab = p_1 \dots p_k q_1 \dots q_l$ is a product of primes.
:::

::: {.theorem #three}
There are infinitely many primes.
:::

::: {.proof name="Euclid 300 BC"}
Suppose there are finitely many primes, say $p_1, \dots, p_k$. Let $N = p_1 \dots p_k + 1$.
Then $p_1 \nmid N$, else $p_1 \mid (N - p_1 \dots p_k) = 1$. 
Clearly $p_1 \mid 1$ is false.
Likewise, none of $p_2, p_3 \dots, p_k$ divide $N$, contradicting the fact that $N$ can be written as a product of primes.
:::

Can a number have more than one factorisation in its primes? Our proof of \@ref(prp:two) does not give uniqueness.

Clearly, $21 = 3 \cdot 7$ is unique.
Why is $9049 \cdot 40099 \neq 6701 \cdot 54151$?

We shall need:

::: {.proposition #four}
If $p$ is a prime and $p \mid ab$ then $p \mid a$ or $p \mid b$.
:::

Proof is later on, just below \@ref(cor:bez).

## Highest Common Factors
:::{.definition #hcf}
Given $a, b \in \mathbb{N}$, a natural number $c$ is the *highest common factor (hcf)*, or *greatest common divisor (gcd)* of $a$ and $b$ if 

i. $c \mid a$ and $c \mid b$ "c is a common divisor of $a$ and $b$"
ii. $d \mid a$ and $d \mid b \implies d \mid c$ "every common factor of $a$ and $b$ divides $c$"

We write $c = \operatorname{hcf}(a, b)$ or $c = \operatorname{gcd}(a, b)$, or simply $c = (a, b)$
\begin{align*}
    \text{E.g. the factors of } &12 \text{ are } 1, 2, 3, 4, 6, 12 \\
    &18 \ \phantom{are} \ 1, 2, 3, 6, 9, 18
\end{align*} 
So the common factors are $1, 2, 3, 6$, hence $\operatorname{hcf}(12, 18) = 6$. 
But if $a$ and $b$ had common factors $1, 2, 3, 4, 6$ then $a$ and $b$ would have no $\operatorname{hcf}$ (according to ii).
Therefore, we will need to show that $\operatorname{hcf}(a, b)$ always exists.
:::

::: {.proposition name="Division Algorithm"}
Let $n, k \in \mathbb{N}$. Then we can write $n = qk + r$, where $q$ and $r$ are integers with $0 \leq r \leq k - 1$.
:::

::: {.proof}
By induction on $n$. True for $n = 1$.

Suppose $n - 1 = q k + r$ for some $q, r \in \mathbb{Z}$, $0 \leq r \leq k - 1$.

If $r < k - 1$ then $n = (n - 1) + 1 = qk + (r + 1)$.

If $r = k - 1$ then $n = (n - 1) + 1 = qk + (k - 1) + 1 = (q + 1)k$.
:::

## Euclid's Algorithm

\begin{array}{c|cc|c}
    \text{INPUT} & a & b & a = 372,\ b = 162 \\
    \hline
    \text{STEP } 1& a = q_1 b + r_1 & q_1, r_1 \in \mathbb{Z} & 372 = 2 \cdot 162 + 48 \\
    & & 0 \leq r \leq b - 1 & \\
    \text{STEP } 2& b = q_2 r_1 + r_2 & 0 \leq r_2 < r_1 & 162 = 3 \cdot 48 + 18 \\
    \text{STEP } 3& r_1 = q_3 r_2 + r_3 & 0 < r_3 < r_2 & 48 = 2 \cdot 18 + 12 \\
    \vdots & \vdots & \vdots & \vdots \\
    \text{STEP } n& r_{n - 2} = q_n r_{n-1} + r_{n} & 0 \leq r_n < r_{n - 1} & 18 = 1 \cdot 12 + 6 \\
    \text{STEP } n + 1& r_{n - 1} = q_{n + 1} r_n + r_{n + 1} & r_{n + 1} = 0 & 12 = 2 \cdot 6 & \\
    \hline
    \text{OUTPUT} & r_n &&&
\end{array} 
Note that the algorithm terminates in $\leq b$ steps, since $b > r_1 > r_2 > \dots \geq 0$.

::: {.theorem}
The output of Euclid's algorithm with input $a, b$ is $\operatorname{hcf}(a, b)$.
:::
::: {.proof}
\ 

i. \begin{align*}
    \text{We can see } &r_n \mid r_{n - 1} \text{ (as } r_{n + 1} = 0 \text{  at STEP } n + 1 \text{)} \\
    \text{so } &r_n \mid r_{n - 2} \ ( \text{STEP } n) \\
    \text{so } &r_n \mid r_i \quad \forall \; i = 1, \dots n - 1 \text{ (by induction)}
\end{align*} 
Hence $r_n \mid b$ (STEP $2$) and $r_n \mid a$ (STEP $1$).

ii. Given $d$ s.t. $d \mid a$ and $d \mid b$,
\begin{align*}
    \text{we have } &d \mid r_1 \text{ (STEP 1) } \\
    \text{so } &d \mid r_2 \text{ (STEP 1) } \\
    \text{so } &d \mid r_i \; \forall \; i = 1, \dots n \text{ (by induction)}
\end{align*} 
Therefore, $r_n = \operatorname{hcf}(a, b)$.
:::

::: {.example}
To obtain $\operatorname{hcf}(87, 52)$ we run Euclid:
\begin{align*}
    87 &= 1(52) + 35 \\
    52 &= 1(35) + 17 \\
    35 &= 2(17) + 1 \\
    17 &= 17(1)
\end{align*} 
so $\operatorname{hcf}(87, 52) = 1$.

When $\operatorname{hcf}(87, 52) = 1$, we also say that $a$ and $b$ are *coprime*.
We can reverse the algorithm:
\begin{align*}
    1 &= 35 - 2 * 17 \\
    &= 35 - 2*(52 - 1(35)) \\
    &= - 2(52) + 3(35) \\
    &= - 2(52) + 3(87 - 1(52)) \\
    &= -5(52) + 3(87)
\end{align*} 
:::

::: {.theorem #seven}
$\forall \; a, b \in \mathbb{N},\ \exists \; x,y \in \mathbb{Z}$ s.t. $xa + yb = \operatorname{hcf}(a, b)$. 
"We can write $\operatorname{hcf}(a, b)$ as a linear combination of $a$ and $b$."
:::

::: {.proof name="1"}
Run Euclid's algorithm with input $a$, $b$, to obtain an output $r_n$. At STEP $n$, we have $r_n = xr_{n-1} + yr_{n-2}$ for some $x, y \in \mathbb{Z}$. 
But $r_{n-1}$ is expressible as $xr_{n-2} + yr_{n-3}$ for some $x, y \in \mathbb{Z}$, from STEP $n-1$, whence $r_n = xr_{n-2} + y r_{n-3}$ for some $x, y \in \mathbb{Z}$. 
Continuing by induction, we have that $\forall \; i = 2, \dots, n-1$, $r_n = xr_i + yr_{i - 1}$ for some $x, y \in \mathbb{Z}$.
Thus $r_n = xa + yb$ for some $x, y \in \mathbb{Z}$, from STEP 1 and 2.
:::

::: {.remark}
Euclid's algorithm not only proves that $x, y \in \mathbb{Z}$, but it gives us a quick way to find them.
:::

::: {.proof name="2"}
Let $h$ be the least positive combination of $a$ and $b$, i.e. the least positive integer of the form $xa + yb$ for some $x, y \in \mathbb{Z}$.

We shall show that $h = \operatorname{hcf}(a, b)$. 

To see (ii) from \@ref(def:hcf), observe that a given $d$ s.t. $d \mid a$ and $d \mid b$, then we have $d \mid ax + by \; \forall \; x, y \in \mathbb{Z}$, so in particular $d \mid h$.

To verify (i), suppose that $h \nmid a$. Then we can write $a = qh + r$ for some $q, r \in \mathbb{Z}$ with $0 < r < h$^[as $h \nmid a$].
Hence $r = a - qh = a - q(xa + yb)$, so $r$ is also a positive linear combination of $a$ and $b$, and strictly smaller than $h$, contradicting the definition of $h$.
Therefore, $h \mid a$ and by the same argument, $h \mid b$.
:::

::: {.remark}
Proof (2) tells us that $\operatorname{hcf}(a,b)$ exists and is a linear combination of $a$ and $b$, *but* gives no way to find $\operatorname{hcf}(a,b)$ or the coefficients $x, y$.
:::

Is there an solution in integers $x, y$ to $320x + 72y = 33$.
No, as LHS is always even but the RHS is odd.

What about $87x + 52y = 33$?
Yes, as we had $x', y' \in \mathbb{Z}$ s.t. $87 x' + 52 y' = 1$, so $x = 33x'$, $y = 33y'$ is an integer solution.

::: {.corollary name="Bezout's Theorem" #bez}
Let $a, b \in \mathbb{N}$. Then the equation $ax + by = c$ has a solution in integers $x, y$ iff $\operatorname{hcf}(a, b) \mid c$.
:::

::: {.proof}
Let $h = \operatorname{hcf}(a, b)$.

Suppose there are $x, y \in \mathbb{Z}$ s.t. $ax + by = c$. Then since $h \mid a$ and $h \mid b$, so $h \mid c$.

Conversely, suppose $h \mid c$. 
But Theorem \@ref(thm:seven) implies that there exist $x, y \in \mathbb{Z}$ s.t. $h = ax + by$.
But then $c = \frac{c}{h} h = \frac{c}{h}(ax + by) = a(x \frac{c}{h}) + b(y \frac{c}{h})$.
:::

We will now give a proof of proposition \@ref(prp:four).

::: {.proof}
Suppose $p \mid ab$ but $p \nmid a$. We will show $p \mid b$. 
Then since $p$ is prime, $\operatorname{hcf}(a, p) = 1$ (as $p \nmid a$).
Thus, by Theorem \@ref(thm:seven), $\exists \; x, y \in \mathbb{Z}$ s.t. $xp + ya = 1$.

It follows that $xpb + yab = b$, $p \mid ab$ so $p \mid b$.
:::

::: {.remark}
\ 

1. Similarly, $p \mid a_1 a_2 \dots a_n \implies p \mid a_i$ for some $i = 1, \dots, n$.
Indeed, Proposition \@ref(prp:four) tells us that if $p \mid a_1 a_2 \dots a_n$, then $p \mid a_1$ or $p \mid a_2 \dots a_n$. 
Proceed by induction on the number of terms in the product.

2. We do need $p$ to be prime.
:::

::: {.theorem name="Fundamental Theorem of Arithmetic" #fta}
Every natural number $n \geq 2$ is expressible as a product of primes, uniquely up to reordering.
:::

::: {.proof}
Existence of factorisation follows from Proposition \@ref(prp:two).
To see uniqueness, use induction on $n$.
True for $n = 2$.

Given $n \geq 2$, suppose $n = p_1 p_2 \dots p_k = q_1 q_2 \dots q_l$, where $p_i, q_j$ are all prime.
We want to show $k = l$ and, after reordering $p_i = q_i \; \forall \; i = 1, \dots, k$.

We have $p_1 \mid n = q_1 q_2 \dots q_l$, so by Proposition \@ref(prp:four), $p_1 \mid q_i$ for some i.
Relabelling the $q_i$, we may assume that $p_1 \mid q_1$.
Since $q_1$ is prime, $p_1 = q_1$.
So $\frac{n}{p_1} = p_2 \dots p_k = q_2 \dots q_l < n$.

By the induction hypothesis, $k = l$, and, after reordering, $p_2 = q_2, \dots, p_k = q_k$.
:::

::: {.remark}
There are "arithmetical systems" (permitting addition, subtraction, multiplication) where factorisation is *not* unique. \
For example, consider $\mathbb{Z}[\sqrt{-3}]$, meaning all complex numbers of the form $x + y \sqrt{-3} = x + y \sqrt{3}i$, where $x, y \in \mathbb{Z}$.
We can add and multiply two elements of $\mathbb{Z}[\sqrt{-3}]$ to get another another element of $\mathbb{Z}[ \sqrt{-3}]$. \
E.g. $(1 + \sqrt{-3}) \cdot (1 - \sqrt{-3}) = 1 + \sqrt{-3} - \sqrt{-3} + 3 = 4$. \
In $Z[ \sqrt{-3} ]$, we can define what it means to be "prime", and both $(1 + \sqrt{-3})$ and $(1 - \sqrt{-3})$ happen to be prime in this sense.
But we can also write $4 = 2 \cdot 2$, so factorisation is not unique. 
:::

## Some Applications of Theorem \@ref(thm:fta)

1. What are the factors of $n = 2^3 \cdot 3^7 \cdot 11$? \
All numbers of the form $2^a 3^b 11^c$, where $0 \leq a \leq 3,\ 0 \leq b \leq 7,\ 0 \leq c \leq 1$.
There are no other factors, for example if $7 \mid n$ then we would have a factorisation of $n$ involving $7$, contradicting uniqueness. \
More generally, the factors of $n = p_1^{a_1} \dots p_k^{a_k}$ are precisely the numbers of the form $p_1^{b_1} \dots p_k^{b_k}$, with $0 \leq b_i \leq a_i \; \forall \; i = 1, \dots, k$.

2. What are the common factors of $2^3 \cdot 3^7 \cdot 5 \cdot 11$ and $2^4 \cdot 3^2 \cdot 11 \cdot 13$? \
All numbers of the form $2^a \cdot 3^b \cdot 5^c \cdot 11^d \cdot 13^e$, where $c = e = 0$ and $0 \leq a \leq 3,\ 0 \leq b \leq 2,\ 0 \leq d \leq 1$. 
Thus the hcf is $2^3 \cdot 3^2 \cdot 11$. \
\
In general, the hcf of $p_1^{a_1} \dots p_k^{a_k}$ and $p_1^{b_1} \dots p_k^{b_k}$, where $a_i, b_i \geq 0$, is $p_1^{\min \{ a_1, b_1 \}} \dots p_k^{\min \{ a_k, b_k \}}$.

3. What are the common multiples of the two numbers in (2)?
All numbers of the form $2^a 3^b 5^c 11^d 13^e$, where $a \geq 4, b \geq 7, c \geq 1, d \geq 3, e \geq 1$, *times* any integer!\
Hence $2^4 3^7 5 11^3 13$ is a common multiple, and any other common multiple is a multiple of it.
We say that it is the *least common multiple* (lcm) of our two numbers. \
\
In general, the lcm of $p_1^{a_1} \dots p_k^{a_k}$ and $p_1^{b_1} \dots p_k^{b_k}$, where $a_i, b_i \geq 0$, is $p_1^{\max \{ a_1, b_1 \}} \dots p_k^{\max \{ a_k, b_k \}}$. \
\
Since $\min \{ a_i, b_i \} + \max \{ a_i, b_i \} = a_i + b_i$, so we have $\operatorname{hcf}(x, y) \cdot \operatorname{lcm}(x, y) = x \cdot y$ for any $x, y$.

4. Another proof of Theorem \@ref(thm:three), due to Erdos (1930): 

::: {.proof}
let $p_1, \dots, p_k$ be primes.
Any number which is a product of just these primes is of the form $p_1^{j_1} p_2^{j_2}, \dots p_k^{j_k} = m^2 p_1^{i_1} p_2^{i_2} \dots p_k^{i_k} (*)$ where $i_x = 0, 1$. \
Let $M \in \mathbb{N}$.
If a number $\leq M$ is of the form $(*)$, then $m^2 \leq M$, i.e. $m \leq \sqrt{M}$.
So there are at most $\sqrt{M} 2^k$ of the form $(*)$ that are $\leq M$.\
If $M > \sqrt{M} 2^k$, i.e $M > 4^k$, then there must be a number $\leq M$ which is *not* of the form $(*)$, which must have a prime factor not amongst $p_1, \dots, p_k$.
::: 

Proof 1 tells us the kth prime is $< 2^{2^k}$. \
Proof 2 tells us kth prime is $< 4^k$. \
In fact, we know kth prime $\sim k \log k$ (Prime Number Theorem).

## Modular arithmetic

Let $n \geq 2$ be a natural number. 
Then the *integers modulo n*, written $\mathbb{Z}_n$ or $\mathbb{Z} / n \mathbb{Z}$, consist of the integers, with two regarded as the same if they differ by a multiple of $n$.
E.g. In $\mathbb{Z}_7$, 2 is the same as 16.
If $x$ and $y$ are the same in $\mathbb{Z}_n$, we write "$x \equiv y \mod n$" (is congruent to) or "$x \equiv y\ (n)$" or "$x = y \text{ in } \mathbb{Z}_n$".
E.g. $2 \equiv 16 \mod 7$
Thus 
\begin{align*}
    x \equiv y \mod n &\iff n \mid x - y \\
    &\iff x = y + k n \text{ for some } k \in \mathbb{Z}
\end{align*} 
We can view $\mathbb{Z}_n$ as
<!--```{r 02-Zn, echo = FALSE, fig.cap = "", fig.align="center", out.width="30%"} 
knitr::include_graphics("figures/02-Zn.png") 
```-->

```{r, echo=FALSE, engine='tikz', fig.ext=if (knitr:::is_latex_output()) 'pdf' else 'png', fig.align = 'center', cache = TRUE,  out.width="250"}
\tikzset{every picture/.style={line width=0.75pt}} %set default line width to 0.75pt        

\begin{tikzpicture}[x=0.75pt,y=0.75pt,yscale=-0.7,xscale=0.7]
%uncomment if require: \path (0,300); %set diagram left start at 0, and has height of 300

%Shape: Circle [id:dp9641223727665371] 
\draw   (200,150) .. controls (200,89.25) and (249.25,40) .. (310,40) .. controls (370.75,40) and (420,89.25) .. (420,150) .. controls (420,210.75) and (370.75,260) .. (310,260) .. controls (249.25,260) and (200,210.75) .. (200,150) -- cycle ;
%Shape: Circle [id:dp4867138741225918] 
\draw  [fill={rgb, 255:red, 184; green, 184; blue, 184 }  ,fill opacity=1 ] (302.5,40) .. controls (302.5,35.86) and (305.86,32.5) .. (310,32.5) .. controls (314.14,32.5) and (317.5,35.86) .. (317.5,40) .. controls (317.5,44.14) and (314.14,47.5) .. (310,47.5) .. controls (305.86,47.5) and (302.5,44.14) .. (302.5,40) -- cycle ;
%Shape: Circle [id:dp6885524539067742] 
\draw  [fill={rgb, 255:red, 184; green, 184; blue, 184 }  ,fill opacity=1 ] (375,67.5) .. controls (375,63.36) and (378.36,60) .. (382.5,60) .. controls (386.64,60) and (390,63.36) .. (390,67.5) .. controls (390,71.64) and (386.64,75) .. (382.5,75) .. controls (378.36,75) and (375,71.64) .. (375,67.5) -- cycle ;
%Shape: Circle [id:dp8052849816078498] 
\draw  [fill={rgb, 255:red, 184; green, 184; blue, 184 }  ,fill opacity=1 ] (410,127.5) .. controls (410,123.36) and (413.36,120) .. (417.5,120) .. controls (421.64,120) and (425,123.36) .. (425,127.5) .. controls (425,131.64) and (421.64,135) .. (417.5,135) .. controls (413.36,135) and (410,131.64) .. (410,127.5) -- cycle ;
%Shape: Circle [id:dp7232843669595623] 
\draw  [fill={rgb, 255:red, 184; green, 184; blue, 184 }  ,fill opacity=1 ] (400,202.5) .. controls (400,198.36) and (403.36,195) .. (407.5,195) .. controls (411.64,195) and (415,198.36) .. (415,202.5) .. controls (415,206.64) and (411.64,210) .. (407.5,210) .. controls (403.36,210) and (400,206.64) .. (400,202.5) -- cycle ;
%Shape: Circle [id:dp14614821359588803] 
\draw  [fill={rgb, 255:red, 184; green, 184; blue, 184 }  ,fill opacity=1 ] (340,252.5) .. controls (340,248.36) and (343.36,245) .. (347.5,245) .. controls (351.64,245) and (355,248.36) .. (355,252.5) .. controls (355,256.64) and (351.64,260) .. (347.5,260) .. controls (343.36,260) and (340,256.64) .. (340,252.5) -- cycle ;
%Shape: Circle [id:dp9823043931092899] 
\draw  [fill={rgb, 255:red, 184; green, 184; blue, 184 }  ,fill opacity=1 ] (260,252.5) .. controls (260,248.36) and (263.36,245) .. (267.5,245) .. controls (271.64,245) and (275,248.36) .. (275,252.5) .. controls (275,256.64) and (271.64,260) .. (267.5,260) .. controls (263.36,260) and (260,256.64) .. (260,252.5) -- cycle ;
%Shape: Circle [id:dp9834315290824136] 
\draw  [fill={rgb, 255:red, 184; green, 184; blue, 184 }  ,fill opacity=1 ] (205,202.5) .. controls (205,198.36) and (208.36,195) .. (212.5,195) .. controls (216.64,195) and (220,198.36) .. (220,202.5) .. controls (220,206.64) and (216.64,210) .. (212.5,210) .. controls (208.36,210) and (205,206.64) .. (205,202.5) -- cycle ;
%Shape: Rectangle [id:dp07149613177907699] 
\draw  [draw opacity=0][fill={rgb, 255:red, 255; green, 255; blue, 255 }  ,fill opacity=1 ] (180,80) -- (250,80) -- (250,160) -- (180,160) -- cycle ;
%Shape: Circle [id:dp5656720700928188] 
\draw  [fill={rgb, 255:red, 184; green, 184; blue, 184 }  ,fill opacity=1 ] (230,67.5) .. controls (230,63.36) and (233.36,60) .. (237.5,60) .. controls (241.64,60) and (245,63.36) .. (245,67.5) .. controls (245,71.64) and (241.64,75) .. (237.5,75) .. controls (233.36,75) and (230,71.64) .. (230,67.5) -- cycle ;

% Text Node
\draw (195.37,127.24) node [anchor=north west][inner sep=0.75pt]  [rotate=-289.59]  {$\dotsc $};
% Text Node
\draw (304,12.4) node [anchor=north west][inner sep=0.75pt]    {$0$};
% Text Node
\draw (391,42.4) node [anchor=north west][inner sep=0.75pt]    {$1$};
% Text Node
\draw (431,112.4) node [anchor=north west][inner sep=0.75pt]    {$2$};
% Text Node
\draw (421,192.4) node [anchor=north west][inner sep=0.75pt]    {$3$};
% Text Node
\draw (351,262.4) node [anchor=north west][inner sep=0.75pt]    {$4$};
% Text Node
\draw (257,262.4) node [anchor=north west][inner sep=0.75pt]    {$5$};
% Text Node
\draw (187,192.4) node [anchor=north west][inner sep=0.75pt]    {$6$};
% Text Node
\draw (164,42.4) node [anchor=north west][inner sep=0.75pt]    {$n\ -\ 1$};
\end{tikzpicture}
```

*Note* If $a \equiv a' \mod n$ and $b \equiv b' \mod n$, then $n \mid (a - a') + (b - b') = (a + b) - (a' + b')$ so $a + b \equiv a' + b' \mod n$. \
Similarly, $n \mid (a - a') \cdot b + (b - b') \cdot a' = ab - a'b'$ so $ab \equiv a'b' \mod n$. \
So we can do *arithmetic* modulo n.

::: {.example}
Does $2a^2 + 3b^3 = 1$ have a solution with $a, b \in \mathbb{Z}$?
:::

*Answer*
If there is a solution, then $2a^2 \equiv 1 \mod 3$, but $2 \cdot 0^2 \equiv 0$, $2 \cdot 1 ^2 \equiv 2$, $2 \cdot 2^2 \equiv 2 \mod 3$.

## Solving congruences
::: {.example}
Solve $7x \equiv 2 \mod 10$.
We note $3 \cdot 7 \equiv 1 \mod 10$, so $3 \cdot 7 x \equiv 3 \cdot 2 \mod 10$ so $x \equiv 6 \mod 10$.
:::

Given $a, b \in \mathbb{Z}$, we say that b is an *inverse of a modulo $n$* if $a b \equiv 1 \mod n$. 
We say $a$ is *invertible modulo $n$*, or is a *unit modulo $n$*, if it has an inverse.
E.g. in $\mathbb{Z}_{10}$, the inverse of $3$ is $7$, and both $3$ and $7$ are units modulo $10$. \
But $4$ is *not* a unit modulo $10$ since $4x \not\equiv 1 \mod 10 \; \forall \; x \in \mathbb{Z}$.

::: {.remark}
If $a$ is a unit modulo $n$ ...

i. ... its inverse is unique (mod $n$). Suppose $\exists \; b, b'$ s.t. $ab \equiv ab' \equiv 1 \mod n$, then $b \equiv bab \equiv bab' \equiv b' \mod n$. 

ii. ... we can write $a^{-1}$ for its inverse.

iii. ... and $ab \equiv ac \mod n$, then $b \equiv c \mod n$.
"We cancel units, multiplying both sides by $a^{-1}$."
This is *not* true in general: $4 \cdot 3 \equiv 4 \cdot 8 \mod 10$ but $3 \not\equiv 8 \mod 10$.
:::

::: {.proposition #ten}
Let $p$ be prime. 
Then every $a \not\equiv 0 \mod p$ is a unit modulo $p$.
:::

::: {.proof}
Have $(a, p) = 1$^[the hcf of $a$ and $p$ is 1], so $\exists \; x, y \in \mathbb{Z}$ s.t. $ax + py = 1$.
Hence $ax = 1 - py$, so $ax \equiv 1 \mod p$ for some $x \in \mathbb{Z}$.
:::

::: {.proposition #tenprime}
Let $n \geq 2$.
Then $a$ is a unit modulo $n$ iff $(a, n) = 1$
:::

::: {.proof}
\begin{align*}
    (a, n) = 1 &\iff ax + ny = 1 \text{ for some } x,y \in \mathbb{Z} \\
    &\iff ax = 1 - ny \text{ for some } x,y \in \mathbb{Z} \\
    &\iff ax \equiv 1 \mod n \text{ for some } x \in \mathbb{Z}.
\end{align*} 
:::

::: {.corollary}
If $(a, n) = 1$, then the congruence $ax \equiv b \mod n$ has a unique solution (mod $n$).
In particular, if $(a, n) = 1$, then there is a unique inverse of $a$, $a^{-1}$, modulo $n$.
Both follow from previous remark.
:::

What if $ax \equiv b \mod n$ with $(a, n) \neq 1$, say $(a, n) = d > 1$? \
Then $n \mid ax - b$ so $d \mid ax - b$ and $d \mid a$, so if there is a solution, then $d \mid b$. \
Conversely, if $d \mid b$, then $n = d \cdot n'$, $a = d \cdot a'$, $b = d \cdot b'$ and
\begin{align*}
    ax \equiv b \mod n &\iff ax - b = kn \text{ for some } k \in \mathbb{Z} \\
    &\iff d \cdot a' \cdot x - d \cdot b' = k \cdot d \cdot n' \text{ for some } k \in \mathbb{Z} \\
    &\iff a' x - b' = k n' \text{ for some } k \in \mathbb{Z} \\
    &\iff a'x \equiv b' \mod n'.
\end{align*} 
Note $(a', b') = 1$. \
So if $(a, n) = d > 1$, the congruence $ax \equiv b \mod n$ has no solutions unless $d \mid b$, in which case the solutions are exactly those of $\frac{a}{d}x \equiv \frac{b}{d} \mod \frac{n}{d}$.

::: {.example}
$7x \equiv 4 \pod {30}$. \
We have $(7, 30) = 1$, so by Euclid $13 \cdot 7 - 3 \cdot 30 = 1$.
Hence $13 \cdot 7 \equiv 1 \mod 30$, whence $x \equiv 4 \cdot 13 \mod 30 = 22 \mod 30$.

Suppose $x'$ is also a solution, that is $7x' \equiv 4 \mod 30$. 
Then $7x \equiv 7x' \mod 30$, so $x \equiv x' \mod 30$ since $7$ is a unit modulo $30$.

*Short form*:
\begin{align*}
    7x &\equiv 4 \mod 30 \\
    \iff 13 \cdot 7 x &\equiv 13 \cdot 4 \mod 30 \quad \text{we have $\Longleftarrow$ since $13$ is a unit modulo $30$} \\
    x &\equiv 22 \mod 30
\end{align*}
:::

::: {.example} 
$10x \equiv 12 \mod 34 \iff 10x = 12 + 34y$
\begin{align*}
    10x \equiv 12 \mod 34 &\iff 10x = 12 + 34y \text{ for some } y \in \mathbb{Z} \\
    &\iff 5x = 6 + 17y \text{ for some } y \in \mathbb{Z} \\
    &\iff 5x \equiv 6 \mod 17 
\end{align*} 
so now we're back in situation 1, and solve this as before.
:::

## Solving simultaneous congruences
\begin{align*}
    \text{Note } x \equiv 5 \mod 12 \implies \begin{cases}
        x \equiv 1 \mod 4 \\
        x \equiv 2 \mod 3
    \end{cases}.
\end{align*} 

Is the converse true, i.e. does $x \equiv 1 \mod 4$ and $x \equiv 2 \mod 3$ imply $x \equiv 5 \mod 12$? \
We inspect 
\begin{align*}
    x &\equiv 1 \mod 4,\ & x &\equiv 1, 5, 9 \mod 12 \\
    x &\equiv 2 \mod 3,\ & x &\equiv 2, 5, 8, 11 \mod 12
\end{align*} 
What about \begin{align*}
    \begin{cases}
        x \equiv 1 \mod 4 \\
        x \equiv 2 \mod 6   
    \end{cases}?
\end{align*} 

::: {.theorem name="Chinese Remainder Theorem" #twelve}
Let $m, n$ be coprime, and $a, b \in \mathbb{Z}$.
Then there is a unique solution modulo $mn$ to the simultaneous equations $x \equiv a \mod m$ and $x \equiv b \mod n$.\
That is, there is a solution $x$ to $x \equiv a \mod m$ and $x \equiv b \mod n$, and y is a solution iff $x \equiv y \mod mn$.
:::

::: {.proof}
Existence:
Since $(m, n) = 1,\; \exists \; s, t \in \mathbb{Z}$ with $sm + tn = 1$.\
Note $sm \equiv 1 \mod n$ as $tn \equiv 0 \mod n$ and $tn \equiv 1 \mod m$ as $sm \equiv 0 \mod m$. \
Hence $x = a(tn) + b(sm) \equiv a \mod m \equiv b \mod n$.

Uniqueness:
Suppose $y$ is also a solution, that is, $y \equiv a \mod m$ and $y \equiv b \mod n$.
\begin{align*}
    &\;\;\; y \equiv a \mod m \text{ and } y \equiv b \mod n \\
    &\iff y \equiv x \mod m \text{ and } y \equiv x \mod n \\
    &\iff m \mid y - x \text { and } n \mid y - x \\
    &\iff mn \mid y - x \hspace{0.5cm} \text{since } (m, n) = 1 \\
    &\iff y \equiv x \mod mn
\end{align*} 
:::

::: {.remark}
Theorem \@ref(thm:twelve) can be extended by induction, to more than two moduli: if $m_1, m_2, \dots, m_k$ are pairwise coprime, then $\forall \; a_1, a_2, \dots, a_k \in \mathbb{Z},\ \exists\; x \in \mathbb{Z}$ s.t.\begin{align*}
    x &\equiv a_1 \mod m_1 \\
    x &\equiv a_2 \mod m_2 \\
    &\;\; \vdots \\
    x &\equiv a_k \mod m_k
\end{align*} 
:::

We denote by $\phi(m)$ the number of integers $a$ s.t. $1 \leq a \leq m$ s.t $(a, m) = 1$, that is, the number of units modulo $m$.
We call $\phi$ the *Euler totient function*.
Define $\phi(1) = 1$. \
E.g. when $p$ is prime, $\phi(p) = p - 1$, and $\phi(p^2) = p^2 - p$ (there are $p$ multiples of $p$ that are $\leq p^2$).\
When $p, q$ are distinct primes, $\phi(pq) = pq - p - q + 1$ (we subtracted $pq$ twice).

## Fermat's Little Theorem

How do powers of an integer behave modulo $p$?

::: {.example}
Modulo $7$, $2^1 \equiv 2$, $2^2 \equiv 4$, $2^3 \equiv 1$, $2^4 \equiv 2$ then repeat $4, 1, 2, 4, 1, 2, \dots$. \
Modulo 11, $2^1 \equiv 2$, $2^2 \equiv 4$, $2^3 \equiv 8$, $2^4 \equiv 5$, $2^5 \equiv 10$, $2^6 \equiv 9$, $2^7 \equiv 7$, $2^8 \equiv 3$, $2^9 \equiv 6$, $2^{10} \equiv 1$ then repeat.
:::

::: {.theorem name="Fermat's Little Theorem" #thirteen}
Let $p$ be a prime.
Then $a^p \equiv a \mod p$ for all $a \in \mathbb{Z}$.
Equivalently, $a^{p-1} \equiv 1 \mod p$ for all $a \not\equiv 0 \mod p$.

Multiply second statement by $a$ and check case of $a \equiv 0 \mod p$ to get first.
$a \not\equiv 0 \mod p$ means $a$ is a unit modulo $p$ and so first statement gives second.
:::

We are going to be a bit general in this proof so we can take the same arguments and apply to composite $p$.

::: {.proof}
If $a \not\equiv 0 \mod p$, then $a$ is a unit mod $p$. \
Thus $ax \equiv ay \mod p$ iff $x \equiv y \mod p$ (multiply by a to go from right to left, and by $a^{-1}$ for converse). 
Hence the numbers $a, 2a, 3a, \dots, (p - 1)a$ are pairwise incongruent (distinct) modulo $p$ and $\not\equiv 0 \mod p$, so they are $1, 2, 3, \dots p - 1$ in some order.

Hence
\begin{align*}
    a \cdot 2a \cdot 3a \cdot \dots \cdot (p - 1)a &\equiv 1 \cdot 2 \cdot 3 \dots \cdot (p - 1) \mod p \\
    a^{p-1} (p - 1)! &\equiv (p - 1)! \mod p. \\
\end{align*} 
But $(p - 1)!$ is a unit mod $p$ (since it is a product of units), so we can cancel it to obtain $a^{p-1} \equiv 1 \mod p$.
:::

::: {.theorem name="Fermat-Euler Theorem" #thirteenprime}
Let $(a, m) = 1$.
Then $a^{\phi(m)} \equiv 1 \mod m$ .
:::

::: {.proof}
Let $U = \{ x \in \mathbb{N} : 0 < x < m : (x, m) = 1 \}$, be the set of units modulo $m$.
Label the elements $u_1, u_2, \dots u_{\phi(m)}$.
Then $a u_1, a u_2, \dots, a u_{\phi(m)}$ are all distinct and invertible modulo $m$ (since $a$ and $u_i$ are units), and hence they are $u_1, u_2, \dots u_{\phi(m)}$ in some order.

It follows that
\begin{align*}
    a u_1 \cdot a u_2 \cdot \dots \cdot a u_{\phi(m)} &\equiv u_1 \cdot u_2 \cdot \dots u_{\phi(m)} \mod m,
\end{align*} 
that is $a^{\phi(m)} z = z \mod m$ where $z = u_1 \cdot u_2 \cdot \dots u_{\phi(m)}$ is a product of units modulo $m$, therefore it itself is a unit.
So we may cancel it to obtain $a^{\phi(m)} = 1 \mod m$ 
:::

## Results about primes

What is $(p - 1)!$ modulo $p$.

::: {.example}
\begin{align*}
    \text{Where } p &= 5,\ 4! = 24 \equiv -1 \mod 5 \\
    p &= 7,\ 6! = 720 \equiv -1 \mod 7
\end{align*} 
:::

::: {.lemma #fourteen}
Let $p$ be prime.
Then $x^2 \equiv 1 \mod p \iff x \equiv \pm 1 \mod p$.
:::

*Note* Modulo $8$, $1^2 = 3^2 = 5^2 = 7^2 = 1$. 
This make us think that $p$ being prime is important.

::: {.proof}
\begin{align*}
    x^2 \equiv 1 \mod p &\iff x^2 - 1 \equiv 0 \mod p \\
    &\iff (x + 1) (x - 1) \equiv 0 \mod p
\end{align*} 
Recall Proposition \@ref(prp:four), if $p$ is prime and $p \mid a b$, then $p \mid a$ or $p \mid b$, so if $p$ is prime, then $ab \equiv 0 \mod p \iff a \equiv 0 \mod p$ or $b \equiv 0 \mod p$.
Hence
\begin{align*}
    x^2 \equiv 1 \mod p &\iff x + 1 \equiv 0 \mod p \text{ or } x - 1 \equiv 0 \mod p \\
    &\iff x \equiv \pm 1 \mod p
\end{align*} 
:::

::: {.remark}
More generally, a non-zero polynomial of degree $k$ over $\mathbb{Z}_p$ has at most k roots.
:::

::: {.theorem #fifteen name="Wilson's Theorem"}
Let $p$ be prime.
Then $(p - 1)! \equiv -1 \mod p$.
:::

::: {.proof}
True for $p = 2$, so assume $p > 2$.\
Note that the units modulo $p$ come in pairs whose product is $1$, together with some elements that are self-inverse, i.e. $x$ s.t. $x^2 \equiv 1 \mod p$.\
But by lemma \@ref(lem:fourteen), the elements of $\mathbb{Z}_p$ that are self-inverse are $+ 1$ and $-1$, so the remaining $p - 3$ elements of $\mathbb{Z}_p$ come in inverse pairs.
[E.g. when $p = 11$, $1, 10$ are self inverses and the pairs are $(2, 6),\ (3, 4),\ (5, 9),\ (7, 8)$].\
Hence $(p - 1)!$ is the product of $\frac{p - 3}{2}$ pairs of inverses together with $+ 1$ and $- 1$, so $(p - 1)! \equiv -1 \mod p$.
:::

When is $-1$ a square modulo $p$? (If ever.)

::: {.example}
When $p = 5, 2^2 \equiv 4 \equiv - 1 \mod 5$.\
When $p = 7, 0^2 = 0, 1^2 = 1, 2^2 = 4, 3^2 = 2 \mod 7$ and we don't need to check $4, 5, 6$ as $(-x)^2 = x^2$.\
When $p = 13, 5^2 \equiv -1 \mod 13$.\
No luck when $p = 19$.
:::

::: {.proposition #sixteen}
Let $p$ be an odd prime.
Then $-1$ is a square modulo $p$ iff $p \equiv 1 \mod 4$.
:::

::: {.proof}
Suppose $p \equiv 1 \mod 4$.
By Wilson's Theorem, \@ref(thm:fifteen),
\begin{align*}
    -1 \equiv (p - 1)! &\equiv 1 \cdot 2 \cdot 3 \cdot \dots \cdot \frac{p - 1}{2} \cdot - \frac{p - 1}{2} \cdot \dots -3 \cdot -2 \cdot -1 \mod p \\
    &\equiv (-1)^{\frac{p-1}{2}} \left( \left(\frac{p-1}{2} \right)! \right)^2 \mod p \\
\end{align*}
But if $p = 4k + 1$ for some $k \in \mathbb{Z}$, then
\begin{align*}
    -1 \equiv (-1)^{2k} \left( (2k)! \right)^2 \mod p
\end{align*} 
so $-1$ is a square mod $p$.

Suppose, on the other hand, that $p \equiv -1 \mod 4$, i.e. $p = 4k + 3$ for some $k \in \mathbb{Z}$.
If $-1$ were a square mod $p$, i.e. if there were $z \in \mathbb{Z}$ s.t. $z^2 \equiv -1 \mod p$, then by Fermat's little Theorem, \@ref(thm:thirteen),
\begin{align*}
    1 \equiv z^{p-1} \equiv z^{4k+2} \equiv z^{2(2k + 1)} &\equiv (-1)^{2k + 1} \mod p \\
    &\equiv -1 \mod p,
\end{align*} 
a contradiction.
:::

::: {.remark}
When $p \equiv 1 \mod 4$, Wilson's Theorem, \@ref(thm:fifteen), tells us a solution to $x^2 \equiv -1 \mod p$.\
E.g. When $p = 29 = 4 \cdot 7 + 1$, $x = (2 \cdot 7)!$ works.
:::

## Public Key Cryptography
Let us agree to write messages as sequences of numbers, e.g. $A \to 00,\ B \to 1, \dots, Z \to 25, ! \to 26, \dots$
I wish for my IA students to be able to send me encrypted messages in such a way that I can decrypt them easily but the same in not true for any third-party observer. 
We use the 

### RSA Scheme (Rivest, Shamir, Adleman)

I think of two large primes $p, q$^[on the order of a hundred digits].
Let $n = pq$, and pick an *encoding exponent* $e$ coprime to $\phi(n) = (p - 1)(q - 1)$.
I publish the pair $(n, e)$ (not the hcf).\
To send me a message (i.e. a sequence of numbers), you chop it into pieces/ numbers $M < n$ and send me $M^e \mod n$, computed quickly by repeated squaring.

To decrypt, I work out $d$ s.t. $ed \equiv 1 \mod \phi(n)$ (by Euclid's algorithm).
Then I compute $(M^e)^d = M^{k \phi(n) + 1}$ for some $k \in \mathbb{Z}$ which is $\equiv M \mod n$ by Fermat-Euler, \@ref(thm:thirteenprime).

Note that in order to decrypt this message in this way, I needed $n$ and $d$, or $n, e$ and $\phi(n)$.
Finding $\phi(n)$ is as hard as finding the prime factors of $n$, which is believed to be computationally hard.\
It is not know if RSA can be broken without factorisation.