# Cosets and Lagrange

::: {.definition}
Let $H \leq G$ and $g \in G$.
The *left coset $gH$* is defined to be $\{ gh : h \in H \}$.
Similarly the *right coset* $Hg = \{ hg : h \in H \}$
:::

::: {.example}
\begin{align*}
    S_3 &= \{ e, \begin{pmatrix}1 & 2 & 3\end{pmatrix}, \begin{pmatrix}1 & 3 & 2\end{pmatrix}, \begin{pmatrix}1 & 2\end{pmatrix}, \begin{pmatrix}1 & 3\end{pmatrix}, \begin{pmatrix}2 & 3\end{pmatrix} \} \\
    H &= \{ \text{id}, \begin{pmatrix}1 & 2 & 3\end{pmatrix}, \begin{pmatrix}1 & 3 & 2\end{pmatrix} \} = A_3 \\
    \begin{pmatrix}1 & 2\end{pmatrix}H &= \left\{ \begin{pmatrix}1 & 2\end{pmatrix}, \begin{pmatrix}1 & 2\end{pmatrix}\begin{pmatrix}1 & 2 & 3\end{pmatrix}, \begin{pmatrix}1 & 2\end{pmatrix}\begin{pmatrix}1 & 3 & 2\end{pmatrix} \right\} \\
    &= \left\{ \begin{pmatrix}1 & 2\end{pmatrix}, \begin{pmatrix}2 & 3\end{pmatrix}, \begin{pmatrix}1 & 3\end{pmatrix} \right\} \\
    \begin{pmatrix}1 & 2 & 3\end{pmatrix}H &= H \ (\text{since H is a subgroup})
\end{align*} 
Note, $H \dot{\cup} \begin{pmatrix}1 & 2\end{pmatrix}H = S_3$
:::

::: {.lemma #nine}
Let $H \leq G$ and $g \in G$.
Then there is a bijection between $H$ and $gH$.
In particular if $H$ is finite then $|H| = |gH|$.
:::

::: {.proof}
Define $\theta_g : H$
\begin{align*}
    \theta_g : H &\to gH \\
    h &\mapsto gh.
\end{align*}
We show $\theta_g$ is a bijection.

Surjectivity: if $gh \in gH$ then $\theta_g(h) = gh$.

Injectivity: \begin{align*}
    \theta_g(h_1) &= \theta_g(h_2) \\
    g h_1 &= g h_2 \\
    \implies h_1 &= h_2 \ (\text{cancellation law})
\end{align*} 
:::

::: {.lemma #ten}
The left cosets of $H$ in $G$ form a partition of $G$ i.e.

i. each $g \in G$ lies in some left coset of $H$ in G.

ii. if $aH \cup bH \neq \emptyset$ (for some $a, b \in G$) $\implies aH = bH$.
:::

```{r 03-cosets, echo = FALSE, fig.cap = "", fig.align="center"} 
knitr::include_graphics("figures/03-cosets.png") 
```

::: {.proof}
\ 

i. $g \in gH$ as $e \in H$

ii. Suppose $c \in aH \cup bH$. \
Claim: $aH = cH = bH$.

Now $c \in aH$ so $c = ak$ for some $k \in H$.
\begin{align*}
    \implies cH &= \{ c h : h \in H \} \\
    &= \{ a k h : h \in H \} \subseteq aH.
\end{align*} 

Similarly, $a = c k^{-1} \in cH$
\begin{align*}
    \implies aH \subseteq cH.
\end{align*} 
So $aH = cH$. \
Similarly $cH = bH$
:::

::: {.example}
$S_n = \underbrace{A_n}_\text{even elements} \dot{\cup} \underbrace{\begin{pmatrix}1 & 2\end{pmatrix} A_n}_\text{odd elements}$
:::

::: {.lemma #eleven}
Let $H \leq G$, $a, b \in G$.
Then $aH = bH \iff a^{-1} b \in H$.
:::

::: {.proof}

$(\implies)$:
\begin{align*}
    b &\in bH = aH \\
    \implies b &= ah \text{ for some } h \in H \\
    \implies a^{-1} b &= h \in H
\end{align*} 

$(\Longleftarrow)$:
\begin{align*}
    \text{Suppose } a^{-1}b &= k \in H \\
    \implies b &= ak \in aH \\
    \text{also } b &\in bH. \\
    \implies aH &= bH
\end{align*} by Lemma \@ref(lem:ten)
:::

::: {.theorem #three name="Lagrange's Theorem"}
Let $H$ be a subgroup of the finite group $G$.
Then the order of $H$ divides the order of $G$ (i.e. $|H| \mid |G|$).
:::

::: {.proof}
a
:::