# Basic Calculus

Basic Calculus - Topic 1.pdf

[test]("Basic Calculus - Topic 1.pdf")

```{r test, echo = FALSE, fig.cap = "", fig.align="center"} 
knitr::include_graphics("Basic Calculus - Topic 1.pdf") 
```

If $f(x) = o(g(x))$ as $x \to x_0$, then $af(x) = o(g(x))$ as $x \to x_0$ for finite $a$.

*Aside*: (Non examinable)


::: {.proof name="Sketch proof of Taylor's Theorem"}
Start from FTC
\begin{align*}
    \int_{0}^{x} f'(t) \,dt &= f(x) - f(0) \\
    \implies f(x) &= f(0) + \int_{0}^{x} f'(t) \,dt \\
    &= f(0) + \int_{0}^{x} \frac{d (t - x)}{d t} * f'(t) \,dt \\
    &= f(0) + [ (t - x) f'(t)]^{t = x}_{t = 0} - \int_{0}^{t} (t - x) f''(t) \,dt \\
    &= f(0) + xf'(0) - \frac{1}{2} \int_{0}^{t} \frac{d (t-x)^2}{d t} f''(t) \,dt \\
    &= f(0) + xf'(0) - \frac{1}{2} [(t-x)^2 f''(t)]^{t = x}_{t = 0} - \int_{0}^{t} + \frac{1}{2} \int_{0}^{t} (t - x)^2 f'''(t) \,dt \\
    &= f(0) + xf'(0) + \frac{1}{2} x^2 f''(0) + \frac{1}{2} \int_{0}^{t} (t - x)^2 f'''(t) \,dt \\
    &\;\;\vdots \\
    &= f(0) + xf'(0) + \frac{x^2}{2!} f''(0) + \ldots + \frac{x^n}{n!} f^{(n)}(0) + \frac{1}{n!} \int_{0}^{x} (t - x)^n f^{(n + 1)}(t) \,dt \\
    &\text{By MVT the remainder = somehow} \\
    &= \frac{x^{(n+1)}}{(n + 1)!} f^{(n + 1)}(x_n) \text{ where } x_n \in [0, x]
\end{align*} 
:::

**3.4.3 Differentiation of an integral with respect to its parameters**

::: {.example}
Suppose we want to evaluate
\begin{align*}
    \int_{0}^{\infty} x^n e^{-x} \,dx \text{ where n is an integer} \\
    \text{Let } I(\lambda) = \int_{0}^{\infty} e^{-\lambda x} \,dx = \frac{1}{\lambda} \\
    \frac{d^n}{d \lambda^n} I = \int_{0}^{\infty} (-x)^n e^{-\lambda x} \,dx = (-1)^n \frac{n!}{\lambda^{n + 1}} \\
    \text{set } \lambda = 1 \text{ and we get } \int_{0}^{\infty} x^n e^{-x} \,dx = n!
\end{align*} 
:::